app roll rev

mirror.v
@@ -64,7 +64,105 @@ Section mirror.
 
 End mirror.
 
+Section bt_list.
+
+  Variables (u x y z : Var) (Hxy : x <> y) (Hux : u <> x) (Huy : u <> y).
+  Variable (f_app f_roll f_rev : Fun).
+
+  Definition fe_app := 
+    MATCH £u WITH 
+         ø⇒ø 
+    OR x#u⇒MATCH £x WITH
+           ø⇒£u
+      OR x#y⇒£x#CALL f_app ON (£y#£u).
+
+  Definition fe_roll := 
+    MATCH £u WITH 
+         ø⇒ø 
+    OR x#y⇒CALL f_app ON (£y#(£x#ø)).
+
+  Definition fe_rev := 
+    MATCH £u WITH 
+         ø⇒ø 
+    OR x#y⇒CALL f_app ON (CALL f_rev ON £y#(£x#ø)).
+
+  Variable (param : Fun -> Var)     
+           (body : Fun -> fun_expr) 
+           (Hparam_app : param f_app = u) (Hbody_app : body f_app = fe_app)
+           (Hparam_roll : param f_roll = u) (Hbody_roll : body f_roll = fe_roll)
+           (Hparam_rev : param f_rev = u) (Hbody_rev : body f_rev = fe_rev).
+
+  Notation "f // s ~~> v" := (fun_sem param body f s v).
+
+  Fact fe_app_spec f e a b : f // e ~~> ⟨a,b⟩ -> CALL f_app ON f // e ~~> bt_app a b.
+  Proof.
+    revert f e; induction a as [ | t _ a IHa ]; intros f e H.
+    + constructor 7 with (1 := H).
+      rewrite Hparam_app, Hbody_app; unfold fe_app.
+      constructor 5 with ω b.
+      { apply fs_var; rew env. }
+      constructor 4.
+      { apply fs_var; rew env. }
+      apply fs_var; rew env.
+    + constructor 7 with (1 := H).
+      rewrite Hparam_app, Hbody_app; unfold fe_app.
+      constructor 5 with ⟨t,a⟩ b.
+      { apply fs_var; rew env. }
+      constructor 5 with t a.
+      { apply fs_var; rew env. }
+      simpl; constructor 3.
+      { apply fs_var; rew env. }
+      apply IHa.
+      constructor 3;
+        apply fs_var; rew env.
+  Qed.
+
+  Fact fe_roll_spec f e a : f // e ~~> a -> CALL f_roll ON f // e ~~> bt_roll a.
+  Proof.
+    destruct a as [ | t a ]; intros H.
+    + constructor 7 with (1 := H).
+      rewrite Hparam_roll, Hbody_roll; unfold fe_roll.
+      constructor 4.
+      { apply fs_var; rew env. }
+      constructor 2.
+    + constructor 7 with (1 := H).
+      rewrite Hparam_roll, Hbody_roll; unfold fe_roll.
+      constructor 5 with t a.
+      { apply fs_var; rew env. }
+      apply fe_app_spec.
+      constructor 3.
+      { apply fs_var; rew env. }
+      constructor 3.
+      { apply fs_var; rew env. }
+      constructor 2.
+  Qed.
+
+  Fact fe_rev_spec f e a : f // e ~~> a -> CALL f_rev ON f // e ~~> bt_rev a.
+  Proof.
+    revert f e; induction a as [ | t _ a IHa ]; intros f e H.
+    + constructor 7 with (1 := H).
+      rewrite Hparam_rev, Hbody_rev; unfold fe_rev.
+      constructor 4.
+      { apply fs_var; rew env. }
+      constructor 2.
+    + constructor 7 with (1 := H).
+      rewrite Hparam_rev, Hbody_rev; unfold fe_rev.
+      constructor 5 with t a.
+      { apply fs_var; rew env. }
+      simpl; apply fe_app_spec.
+      constructor 3.
+      * apply IHa.
+        apply fs_var; rew env.
+      * constructor 3.
+        { apply fs_var; rew env. }
+        constructor 2.
+  Qed.
+
+End bt_list.
+
 Local Notation "f // e ~~> v [ p , b ]" := (fun_sem p b f e v) (at level 70, format "f  //  e  ~~>  v  [ p , b ]", no associativity).
 
 Check fe_mirror_spec.
+Check fe_roll_spec.
+Check fe_rev_spec.
 
